site/widgets/ai/learned_middle_block_recurrence.js
@@ -2,7 +2,7 @@ import { mod, positiveInt } from "../shared/circle_math_core.js";
 import { addLabeledNumber, addOutput, addWidgetHeader, clear } from "../shared/svg_helpers.js";
 import { loadJson, mountWidgets, statusClass, statusLabel } from "../shared/widget_base.js";
 
-const THEOREM_IDS = ["AIM-T0006", "AIM-T0007", "AIM-T0008", "AIM-T0009", "AIM-T0018"];
+const THEOREM_IDS = ["AIM-T0006", "AIM-T0007", "AIM-T0008", "AIM-T0009", "AIM-T0018", "AIM-T0039", "AIM-T0040", "AIM-T0041", "AIM-T0042", "AIM-T0043"];
 const DICTIONARY_IDS = ["COMMON-0052", "COMMON-0053", "COMMON-0059", "COMMON-0068", "COMMON-0070"];
 
 let chartIdCounter = 0;
